implementation of mappings by rbts

src/HOL/Library/Table.thy
@@ -3,7 +3,7 @@
 header {* Tables: finite mappings implemented by red-black trees *}
 
 theory Table
-imports Main RBT
+imports Main RBT Mapping
 begin
 
 subsection {* Type definition *}
@@ -23,7 +23,8 @@ lemma table_eq:
   "t1 = t2 \<longleftrightarrow> tree_of t1 = tree_of t2"
   by (simp add: tree_of_inject)
 
-code_abstype Table tree_of
+lemma [code abstype]:
+  "Table (tree_of t) = t"
   by (simp add: tree_of_inverse)
 
 
@@ -55,6 +56,9 @@ lemma tree_of_delete [code abstract]:
 
 definition entries :: "('a\<Colon>linorder, 'b) table \<Rightarrow> ('a \<times> 'b) list" where
   [code]: "entries t = RBT.entries (tree_of t)"
+
+definition keys :: "('a\<Colon>linorder, 'b) table \<Rightarrow> 'a list" where
+  [code]: "keys t = RBT.keys (tree_of t)"
 
 definition bulkload :: "('a\<Colon>linorder \<times> 'b) list \<Rightarrow> ('a, 'b) table" where
   "bulkload xs = Table (RBT.bulkload xs)"
@@ -101,6 +105,10 @@ lemma entries_tree_of:
   "RBT.entries (tree_of t) = entries t"
   by (simp add: entries_def)
 
+lemma keys_tree_of:
+  "RBT.keys (tree_of t) = keys t"
+  by (simp add: keys_def)
+
 lemma lookup_empty [simp]:
   "lookup empty = Map.empty"
   by (simp add: empty_def lookup_Table expand_fun_eq)
@@ -111,15 +119,19 @@ lemma lookup_update [simp]:
 
 lemma lookup_delete [simp]:
   "lookup (delete k t) = (lookup t)(k := None)"
-  by (simp add: delete_def lookup_Table lookup_delete lookup_tree_of restrict_complement_singleton_eq)
+  by (simp add: delete_def lookup_Table RBT.lookup_delete lookup_tree_of restrict_complement_singleton_eq)
 
 lemma map_of_entries [simp]:
   "map_of (entries t) = lookup t"
   by (simp add: entries_def map_of_entries lookup_tree_of)
 
+lemma entries_lookup:
+  "entries t1 = entries t2 \<longleftrightarrow> lookup t1 = lookup t2"
+  by (simp add: entries_def lookup_def entries_lookup)
+
 lemma lookup_bulkload [simp]:
   "lookup (bulkload xs) = map_of xs"
-  by (simp add: bulkload_def lookup_Table lookup_bulkload)
+  by (simp add: bulkload_def lookup_Table RBT.lookup_bulkload)
 
 lemma lookup_map_entry [simp]:
   "lookup (map_entry k f t) = (lookup t)(k := Option.map f (lookup t k))"
@@ -133,7 +145,85 @@ lemma fold_fold:
   "fold f t = (\<lambda>s. foldl (\<lambda>s (k, v). f k v s) s (entries t))"
   by (simp add: fold_def expand_fun_eq RBT.fold_def entries_tree_of)
 
+lemma is_empty_empty [simp]:
+  "is_empty t \<longleftrightarrow> t = empty"
+  by (simp add: table_eq is_empty_def tree_of_empty split: rbt.split)
+
+lemma RBT_lookup_empty [simp]: (*FIXME*)
+  "RBT.lookup t = Map.empty \<longleftrightarrow> t = RBT.Empty"
+  by (cases t) (auto simp add: expand_fun_eq)
+
+lemma lookup_empty_empty [simp]:
+  "lookup t = Map.empty \<longleftrightarrow> t = empty"
+  by (cases t) (simp add: empty_def lookup_def Table_inject Table_inverse)
+
+lemma sorted_keys [iff]:
+  "sorted (keys t)"
+  by (simp add: keys_def RBT.keys_def sorted_entries)
+
+lemma distinct_keys [iff]:
+  "distinct (keys t)"
+  by (simp add: keys_def RBT.keys_def distinct_entries)
+
+
+subsection {* Implementation of mappings *}
+
+definition Mapping :: "('a\<Colon>linorder, 'b) table \<Rightarrow> ('a, 'b) mapping" where
+  "Mapping t = Mapping.Mapping (lookup t)"
+
+code_datatype Mapping
+
+lemma lookup_Mapping [simp, code]:
+  "Mapping.lookup (Mapping t) = lookup t"
+  by (simp add: Mapping_def)
+
+lemma empty_Mapping [code]:
+  "Mapping.empty = Mapping empty"
+  by (rule mapping_eqI) simp
+
+lemma is_empty_Mapping [code]:
+  "Mapping.is_empty (Mapping t) \<longleftrightarrow> is_empty t"
+  by (simp add: table_eq Mapping.is_empty_empty Mapping_def)
+
+lemma update_Mapping [code]:
+  "Mapping.update k v (Mapping t) = Mapping (update k v t)"
+  by (rule mapping_eqI) simp
+
+lemma delete_Mapping [code]:
+  "Mapping.delete k (Mapping xs) = Mapping (delete k xs)"
+  by (rule mapping_eqI) simp
+
+lemma keys_Mapping [code]:
+  "Mapping.keys (Mapping t) = set (keys t)"
+  by (simp add: keys_def Mapping_def Mapping.keys_def lookup_def lookup_keys)
+
+lemma ordered_keys_Mapping [code]:
+  "Mapping.ordered_keys (Mapping t) = keys t"
+  by (rule sorted_distinct_set_unique) (simp_all add: ordered_keys_def keys_Mapping)
+
+lemma Mapping_size_card_keys: (*FIXME*)
+  "Mapping.size m = card (Mapping.keys m)"
+  by (simp add: Mapping.size_def Mapping.keys_def)
+
+lemma size_Mapping [code]:
+  "Mapping.size (Mapping t) = length (keys t)"
+  by (simp add: Mapping_size_card_keys keys_Mapping distinct_card)
+
+lemma tabulate_Mapping [code]:
+  "Mapping.tabulate ks f = Mapping (bulkload (List.map (\<lambda>k. (k, f k)) ks))"
+  by (rule mapping_eqI) (simp add: map_of_map_restrict)
+
+lemma bulkload_Mapping [code]:
+  "Mapping.bulkload vs = Mapping (bulkload (List.map (\<lambda>n. (n, vs ! n)) [0..<length vs]))"
+  by (rule mapping_eqI) (simp add: map_of_map_restrict expand_fun_eq)
+
+lemma [code, code del]: "HOL.eq (x :: (_, _) mapping) y \<longleftrightarrow> x = y" by (fact eq_equals) (*FIXME*)
+
+lemma eq_Mapping [code]:
+  "HOL.eq (Mapping t1) (Mapping t2) \<longleftrightarrow> entries t1 = entries t2"
+  by (simp add: eq Mapping_def entries_lookup)
+
 hide (open) const tree_of lookup empty update delete
-  entries bulkload map_entry map fold
+  entries keys bulkload map_entry map fold
 
 end
